src/int.v
@@ -974,13 +974,6 @@ Definition ITER_DOWN {S}
 :=
   ITER (step_down i k) k (complete_down i k) body loop.
 
-Definition ITERX_DOWN {S A}
-  (i k : nat)
-  (body : int → nat → S → WP (S * option A))
-  (loop : S → WP (S * option A))
-:=
-  ITERX (step_down i k) i (complete_down i k) body loop.
-
 (* In this variant, the loop indices [_k] and [_i] are explicitly passed
    as arguments to the loop. [loop _k _i s Q] means that the loop, applied
    to the extremum indices [_k] and [_i] and to the initial state [s],
@@ -1038,13 +1031,6 @@ Definition ITER_UP {S}
   (loop : S → WP S)
 :=
   ITER (step_up i k) i (complete_up i k) body loop.
-
-Definition ITERX_UP {S A}
-  (i k : nat)
-  (body : int → nat → S → WP (S * option A))
-  (loop : S → WP (S * option A))
-:=
-  ITERX (step_up i k) i (complete_up i k) body loop.
 
 (* In this variant, the loop indices [_i] and [_k] are explicitly passed
    as arguments to the loop. [loop _i _k s Q] means that the loop, applied
@@ -1284,108 +1270,6 @@ Global Ltac wp_iter_up I :=
 
 (* -------------------------------------------------------------------------- *)
 
-(* An interruptible loop, counting up from [a] to [b]. The loop can be
-   broken via an early exit: the loop body [f] returns an instruction to
-   either continue or stop (break). *)
-
-Section InterruptibleUpAux.
-Context {S A : Type}.
-Implicit Types _a : int.
-Implicit Types s : S.
-
-(* We hoist the loop-invariant parameters out of the loop, because
-   otherwise Equations produces ugly code where these parameters are
-   carried around in a tuple, itself encoded using nested pairs. *)
-
-Variable _b : int.
-Variable f : int → S → S * option A.
-
-(* [interruptible_up_aux _a s] applies the loop body [f] to every machine
-   integer from [_a], included, up to [_b], excluded. A state of type [S]
-   is carried, whose initial value is [s]. If [f] returns [break x] then
-   the loop stops and returns the pair [(s, break x)] where [s] is the
-   current state. If [f] returns [continue] then the loop continues. If
-   [f] never returns [break _] then the loop runs all the way to the end
-   and returns [(s, continue)] where [s] is the final state. *)
-
-(* Another possible convention for an interruptible loop would be to
-   assume that the loop-carried state contains the continuation flag
-   (i.e., the state typically has type [S * option A]) and to let the
-   user provide a function that inspects the current state and
-   determines whether the loop should continue or stop. *)
-
-Equations interruptible_up_aux _a s : S * option A
-by wf _a igt :=
-interruptible_up_aux _a s with inspect (_a <? _b)%uint63 => {
-| inspected true :=
-    do so ← f _a s ;
-    let '(s, o) := so in
-    match o with
-    | continue =>
-        interruptible_up_aux (_a+1)%uint63 s
-    | break _ =>
-        so
-    end
-| inspected false :=
-    (s, continue)
-}.
-Next Obligation.
-  eauto using safe_increment'.
-Qed.
-
-End InterruptibleUpAux.
-
-Section InterruptibleUp.
-Context {S A : Type}.
-Implicit Types _a _b : int.
-Implicit Types s : S.
-Implicit Types f : int → S → S * option A.
-
-(* A specification of [interruptible_up_aux]. *)
-
-Lemma wp_interruptible_up_aux f :
-  ∀ _a a _b b ,
-  isInt _a a →
-  isInt _b b →
-  representable a →
-  representable b →
-  ITERX_UP
-    a b
-    (λ _j j s Q, a ≤ j < b → representable j → wp (f _j s) Q)
-    (λ s Q, wp (interruptible_up_aux _b f _a s) Q).
-Proof.
-  intros. ITER.
-  funelim (interruptible_up_aux _b f _a s); cleanup; clear Heqcall;
-  isBool_magic; autorewrite with nat.
-  (* [funelim] creates an induction hypothesis that contains
-     spurious parameters of type [S * option A] and [option A]. *)
-  assert (dummy: option A). { exact continue. }
-  (* Case [a < b]. *)
-  { wp_op Hstep s'. clear dependent s. destruct s' as [ s [x|] ].
-    (* Subcase: [out] is [break x]. *)
-    + wp_ret. eauto with lia.
-    (* Subcase: [out] is [continue]. *)
-    + eapply wp_conseq.
-      - eapply H; itc.
-      - autorewrite with nat. eauto. }
-  (* Case [b ≤ a]. *)
-  { wp_ret. eauto with lia. }
-Qed.
-
-(* A definition of [interruptible_up], with reordered parameters. *)
-
-Definition interruptible_up _a _b s f :=
-  interruptible_up_aux _b f _a s.
-
-(* Copying the specification of [interruptible_up_aux],
-   to obtain a specification of [interruptible_up],
-   would be useless; they are the same up to the order of parameters. *)
-
-Definition wp_interruptible_up :=
-  wp_interruptible_up_aux.
-
-End InterruptibleUp.
-
 (* This lemma can help prove that a loop invariant can be extended. *)
 
 (* Unfortunately, [eauto] refuses to use it as a hint, and I am also
@@ -1441,9 +1325,9 @@ Lemma wp_walk_up_aux :
   representable a →
   isInt _b b →
   representable b →
-  ITERX_CPS
+  XITER
     (step_up a b) a (complete_up a b)
-    (λ _j j s W normal exit Q, wp (body _j s normal exit) Q)
+    (λ _ _j j s normal exit Q, wp (body _j s normal exit) Q)
     (λ s Q, wp (walk_up_aux _a s) Q).
 Proof.
   (* The spec is quite complex, but the proof is very simple. *)
@@ -1509,7 +1393,7 @@ Lemma wp_uxiter_up_aux :
   representable a →
   isInt _b b →
   representable b →
-  ITERXU_CPS
+  UXITER
     (step_up a b) a (complete_up a b)
     (λ _j j _ normal exit Q, wp (body _j normal exit) Q)
     (λ Q, wp (uxiter_up_aux _a) Q).
@@ -1539,93 +1423,3 @@ Definition uxiter_up {A} _a _b
 (* TODO define a tactic *)
 Definition wp_uxiter_up :=
   @wp_uxiter_up_aux.
-
-(* -------------------------------------------------------------------------- *)
-
-(* A variant of [interruptible_up] that does not carry a state. *)
-
-Section InterruptibleUpUnitAux.
-Context {A : Type}.
-Implicit Types _a : int.
-
-Variable _b : int.
-Variable f : int → option A.
-
-Equations interruptible_up_unit_aux _a : option A
-by wf _a igt :=
-interruptible_up_unit_aux _a with inspect (_a <? _b)%uint63 => {
-| inspected true :=
-    do o ← f _a ;
-    match o with
-    | continue =>
-        interruptible_up_unit_aux (_a+1)%uint63
-    | break _ =>
-        o
-    end
-| inspected false :=
-    continue
-}.
-Next Obligation.
-  eauto using safe_increment'.
-Qed.
-
-End InterruptibleUpUnitAux.
-
-(* Instead of proving a specification of [interruptible_up_unit_aux],
-   we first prove that it is related with [interruptible_up_aux]. *)
-
-(* The relation is [wus], which stands for [with_unit_state]. *)
-
-Definition wus {A} (a : A) (sa' : unit * A) :=
-  a =
-    do sa' ← sa' ;
-    let '(s', a') := sa' in
-    a'.
-
-Lemma interruptible_up_unit_aux_eq {A} _a _b
-  (f : int → option A)
-  (f' : int → unit → unit * option A) :
-  (∀ _i, wus (f _i) (f' _i tt)) →
-  wus
-    (interruptible_up_unit_aux _b f _a)
-    (interruptible_up_aux _b f' _a tt).
-Proof.
-  intros Hf.
-  funelim (interruptible_up_unit_aux _b f _a); cleanup; clear Heqcall;
-  autorewrite with interruptible_up_aux; simpl; rewrite e.
-  (* [funelim] introduces a spurious parameter: *)
-  assert (dummy: option A). { exact continue. }
-  { rewrite Hf. destruct (f' _a ()) as [ [] [|] ]; unfold bind.
-    + unfold wus. eauto.
-    + eauto. }
-  { unfold wus. eauto. }
-Qed.
-
-Section InterruptibleUpUnit.
-Context {A : Type}.
-Implicit Types _a _b : int.
-Implicit Types f : int → option A.
-
-Definition interruptible_up_unit _a _b f :=
-  interruptible_up_unit_aux _b f _a.
-
-End InterruptibleUpUnit.
-
-(* When used with [rewrite], the following lemma allows replacing a call
-   to [interruptible_up_unit] with a call to [interruptible_up]. *)
-
-Lemma interruptible_up_unit_eq {A} _a _b (f : int → option A) :
-  wus
-    (interruptible_up_unit _a _b f)
-    (interruptible_up _a _b tt (λ _i s, do o ← f _i ; (s, o))).
-Proof.
-  intros.
-  unfold interruptible_up_unit, interruptible_up.
-  eapply interruptible_up_unit_aux_eq.
-  unfold wus, bind. eauto.
-Qed.
-
-(* We do not provide a specification of [interruptible_up_unit].
-   Instead, the user is expected to rewrite using the above lemma
-   and to use the specification of [interruptible_up]. This can
-   introduce a little noise in the proof, but seems bearable. *)
